@@ -3,34 +3,58 @@ import Chartreux.Duke.Defs
 variable {ID : Type}
 variable [DecidableEq ID]
 
-def State := ID -> Option Val
+inductive StateEntry where
+| unknown
+| declared (v : Option Val)
+
+def State := ID -> StateEntry
 abbrev NState := @State Nat
 abbrev SState := @State String
 @[simp]
-def State.set (σ : @State ID) (x : ID) (v : Option Val) : @State ID :=
+def State.set (σ : @State ID) (x : ID) (v : StateEntry) : @State ID :=
   fun y => if x = y then v else σ y
-def State.declared (σ : @State ID) (x : ID) : @State ID := σ.set x none
-def State.updated (σ : @State ID) (x : ID) (v : Val) : @State ID := σ.set x v
-def State.empty : @State ID := fun _ => none
+def State.declared (σ : @State ID) (x : ID) : Option (@State ID) :=
+  match σ x with
+  | .unknown => some (σ.set x (.declared none))
+  | .declared _ => none
+def State.updated (σ : @State ID) (x : ID) (v : Val) : Option (@State ID) :=
+  match σ x with
+  | .unknown => none
+  | .declared _ => some (σ.set x (.declared v))
+def State.empty : @State ID := fun _ => .unknown
 def State.isInit (σ : @State ID) : Prop := σ = State.empty
 
 namespace State
 
-theorem updated_eq {σ : @State ID} {x : ID} {v : Val} :
-    σ.updated x v x = some v := by
-  simp [State.updated] at *
-
-theorem declared_eq {σ : @State ID} {x : ID} :
-    σ.declared x x = none := by
+theorem declared_eq {σ σ' : @State ID} {x : ID} :
+    σ.declared x = some σ' -> σ' x = .declared none := by
   simp [State.declared] at *
+  split <;> simp
+  intro rfl
+  cbv
 
-theorem declared_neq  {σ : @State ID} {x y : ID} (hne : x ≠ y) :
-    σ.declared x y = σ y := by
+theorem updated_eq {σ σ' : @State ID} {x : ID} {v : Val} :
+    σ.updated x v  = some σ' -> σ' x = .declared v := by
+  simp [State.updated] at *
+  split <;> simp
+  intro rfl
+  cbv
+
+theorem declared_neq  {σ σ' : @State ID} {x y : ID} (hne : x ≠ y) :
+    σ.declared x = some σ' -> σ' y = σ y := by
   simp [State.declared, *]
+  split <;> simp
+  intro rfl
+  simp
+  grind
 
-theorem updated_neq  {σ : @State ID} {x y : ID} {v : Val} (hne : x ≠ y) :
-    σ.updated x v y = σ y := by
+theorem updated_neq  {σ σ' : @State ID} {x y : ID} {v : Val} (hne : x ≠ y) :
+    σ.updated x v = some σ' -> σ' y = σ y := by
   simp [State.updated, *]
+  split <;> simp
+  intro rfl
+  simp
+  grind
 
 end State
 
@@ -48,7 +72,7 @@ inductive EvalExpr (σ : State) : @Expr ID -> Val -> Prop where
 | int : ∀ n,
     EvalExpr σ (.Int n) (.Int n)
 | var : ∀ x v,
-    σ x = some v ->
+    σ x = .declared (some v) ->
     EvalExpr σ (.Var x) v
 | isnullT : ∀ e,
     EvalExpr σ e (.Null) ->
